\documentclass{article}
\usepackage{amssymb,amsmath}
\usepackage{mathtools}
\usepackage{graphicx}
\usepackage{multicol}
\usepackage{array}
\topmargin=-0.3in
\textheight=9.2in
\textwidth=168mm
\oddsidemargin=-0.2in
\evensidemargin=-0.2in
\begin{document}
\section*{General Solutions To IBVP's}
\subsubsection*{The Heat Equation}
\[
\begin{array}{c c}
\begin{cases}
u_{t} - ku_{xx} = 0\\
u(0,t) = u(L,t) = 0\\
u(x,0) = f(x)
\end{cases}
&
\begin{cases}
u_{t} - ku_{xx} = 0\\
u_{x}(0,t) = u_{x}(L,t) = 0\\
u(x,0) = g(x)
\end{cases}\\
&\\
u(x,t) = \sum_{n=1}^{\infty}e^{-k\left(\frac{n\pi}{L}\right)^{2}t}\sin{\left(\frac{n\pi x}{L}\right)}
& u(x,t) = \frac{a_{0}}{2} + \sum_{n=1}^{\infty}e^{-k\left(\frac{n\pi}{L}\right)^{2}t}\cos{\left(\frac{n\pi x}{L}\right)}\\
&\\
\begin{cases}
u_{t} - ku_{xx} = 0\\
u(0,t) = u_{x}(L,t) = 0\\
u(x,0) = h(x)
\end{cases}
&
\begin{cases}
u_{t} - ku_{xx} = 0\\
u_{x}(0,t) = u(L,t) = 0\\
u(x,0) = k(x)
\end{cases}\\
&\\
u(x,t) =  \sum_{n=1}^{\infty}e^{-k\left(\left[n + \frac{1}{2}\right]\frac{\pi}{L}\right)^{2}t}\sin{\left(\left[n + \frac{1}{2}\right]\frac{\pi x}{L}\right)}
& u(x,t) =  \sum_{n=1}^{\infty}e^{-k\left(\left[n + \frac{1}{2}\right]\frac{\pi}{L}\right)^{2}t}\cos{\left(\left[n + \frac{1}{2}\right]\frac{\pi x}{L}\right)}
\end{array}
\]
\noindent\\
\subsubsection*{The Wave Equation}
\[
\begin{array}{c c}
\begin{cases}
u_{tt} - c^{2}u_{xx} = 0\\
u(0,t) = u(L,t) = 0\\
u(x,0) = f(x) \quad u_{t}(x,0) = g(x)
\end{cases}
&
\begin{cases}
u_{tt} - c^{2}u_{xx} = 0\\
u_{x}(0,t) = u_{x}(L,t) = 0\\
u(x,0) = f(x) \quad u_{t}(x,0) = g(x)
\end{cases}\\
&\\
u(x,t) = \sum_{n=1}^{\infty}\left[a_{n}\cos{\left(\frac{n \pi t c}{L}\right)} + b_{n}\sin{\left(\frac{n \pi t c}{L}\right)}\right]\sin{\left(\frac{n \pi x}{L}\right)}
&u(x,t) = \frac{a_{0}}{2} + \sum_{n=1}^{\infty}\left[a_{n}\cos{\left(\frac{n \pi t c}{L}\right)} + b_{n}\sin{\left(\frac{n \pi t c}{L}\right)}\right]\cos{\left(\frac{n \pi x}{L}\right)}\\
&\\
\end{array}
\]
\[
\begin{array}{c}
\begin{cases}
u_{tt} - c^{2}u_{xx} = 0\\
u(0,t) = u_{x}(L,t) = 0\\
u(x,0) = f(x) \quad u_{t}(x,0) = g(x)
\end{cases}\\
\\
u(x,t) = a_{0} + b_{0}t + \sum_{n=1}^{\infty}\left[ a_{n}\cos{\left(\left[n + \frac{1}{2}\right]\frac{\pi t}{L}\right)} + b_{n}\sin{\left(\left[n + \frac{1}{2}\right]\frac{\pi x}{L}\right)}\right]\sin{\left(\left[n + \frac{1}{2}\right]\frac{\pi x}{L}\right)}\\
\\
\begin{cases}
u_{tt} - c^{2}u_{xx} = 0\\
u_{x}(0,t) = u(L,t) = 0\\
u(x,0) = f(x) \quad u_{t}(x,0) = g(x)
\end{cases}\\
\\
u (x,t) = a_{0} + b_{0}t + \sum_{n=1}^{\infty}\left[ a_{n}\cos{\left(\left[n + \frac{1}{2}\right]\frac{\pi t}{L}\right)} + b_{n}\sin{\left(\left[n + \frac{1}{2}\right]\frac{\pi x}{L}\right)}\right]\cos{\left(\left[n + \frac{1}{2}\right]\frac{\pi x}{L}\right)}
\end{array}
\]
\subsubsection*{The Laplace Equation}
\paragraph{\indent Cartesian Coordinates}
\[
\begin{array}{c c}
\begin{cases}
u_{xx} + u_{yy} = 0\\
u(0,y) = u(L,y) = 0
\end{cases}
&
\begin{cases}
u_{xx} + u_{yy} = 0\\
u_{x}(0,y) = u_{x}(L,y) = 0
\end{cases}\\
&\\
u(x,y) = \sum_{n=1}^{\infty}\left[a_{n}\sinh{\left(\frac{n \pi y}{L}\right)} + b_{n}\cosh{\left(\frac{n\pi y}{L}\right)}\right]\sin{\left(\frac{n\pi x}{L}\right)}
& u(x,y) = \sum_{n=1}^{\infty}\left[a_{n}\sinh{\left(\frac{n \pi y}{L}\right)} + b_{n}\cosh{\left(\frac{n\pi y}{L}\right)}\right]\cos{\left(\frac{n\pi x}{L}\right)}
\end{array}
\]
\\
\[
\begin{array}{c}
\begin{cases}
u_{xx} + u_{yy} = 0\\
u_{x}(0,y) = u(L,y) = 0
\end{cases}\\
\\
u(x,t) = \sum_{n=1}^{\infty}\left[a_{n}\sinh{\left(\left[n + \frac{1}{2}\right]\frac{\pi y}{L}\right)} + b_{n}\cosh{\left(\left[n + \frac{1}{2}\right]\frac{\pi y}{L}\right)}\right]\cos{\left(\left[n + \frac{1}{2}\right]\frac{\pi y}{L}\right)}\\
\\
\begin{cases}
u_{xx} + u_{yy} = 0\\
u(0,y) = u_{x}(L,y) = 0
\end{cases}\\
\\
u(x,t) = \sum_{n=1}^{\infty}\left[a_{n}\sinh{\left(\left[n + \frac{1}{2}\right]\frac{\pi y}{L}\right)} + b_{n}\cosh{\left(\left[n + \frac{1}{2}\right]\frac{\pi y}{L}\right)}\right]\sin{\left(\left[n + \frac{1}{2}\right]\frac{\pi y}{L}\right)}
\end{array}
\]
\paragraph{\indent Polar Coordinates}
\begin{gather*}
\begin{cases}
u_{rr} + \frac{1}{r}u_{r} + \frac{1}{r^{2}}u_{\theta\theta} = 0\\
u(h,\theta) = f(\theta)\quad \text{on}\ x < \theta < L
\end{cases}\\
u(r,\theta) = a_{0} + \sum_{n=1}^{\infty}a_{n}r^{n}\cos{\left(\frac{n \pi \theta}{L}\right)} + b_{n}r^{n}\sin{\left(\frac{n \pi \theta}{L}\right)}
\end{gather*}
\end{document}