\documentclass{article}
\usepackage{amssymb,amsmath}
\usepackage{mathtools}
\usepackage{array}
\topmargin=-0.3in
\textheight=9.2in
\textwidth=168mm
\oddsidemargin=-0.2in
\evensidemargin=-0.2in
\title{Test 1 Solutions}
\date{}

\newcommand{\ut}{u_{t}}
\newcommand{\utt}{u_{tt}}
\newcommand{\uxx}{u_{xx}}
\newcommand{\ux}{u_{x}}
\newcommand{\uy}{u_{y}}
\newcommand{\uyy}{u_{yy}}

\newcommand{\dx}{\mathop{dx}}
\newcommand{\dy}{\mathop{dy}}
\newcommand{\dt}{\mathop{dt}}
\newcommand{\pt}{\partial}

\begin{document}
\begin{enumerate}
\item Solve the first order Cauchy problem
\[
\begin{cases}
\ut + \ux - 3u = t\\
u(x,0) = x^{2}
\end{cases}
\]
From the coefficients on the $\ut$ and $\ux$, we know that
\begin{gather*}
\frac{\dx}{\dt} = 1\\
\int \dx = \int \dt\\
x = t + c\\
x- t = c.
\end{gather*}
Now we need to find our substitutions $s$ and $w$.
If we let $s = x-t$, then we can arbitrarily let $w = t$.
Now we need to find $\ut$ and $\ux$.

\begin{minipage}[t]{0.5\textwidth}
\begin{align*}
\ut &= u_{s}\frac{\pt s}{\pt t} + u_{w}\frac{\pt w}{\pt t}\\
&= -u_{s} + u_{w}\\
&= u_{w} - u_{s}
\end{align*}
\end{minipage}
\begin{minipage}[t]{0.5\textwidth}
\begin{align*}
\ux &= u_{s}\frac{\pt s}{\pt x} + u_{w}\frac{\pt w}{\pt x}\\
&= u_{s}
\end{align*}
\end{minipage}
Now we substitute back into our originial equation.
\begin{align*}
-u_{s} + u_{w} + u_{s} - 3u &= w\\
u_{w} - 3u &= w
\end{align*}
We now have a first order ODE that we can solve by
\begin{gather*}
y' - 3y = x\\
y_{g} = c_{1}e^{3x} \qquad\qquad\qquad\qquad y_{p} = \frac{1}{3}x - \frac{1}{9}\\
y = c_{1}e^{3x} + \frac{1}{3}x - \frac{1}{9}\\
u(s,w) = f(s)e^{3w} + \frac{1}{3}w - \frac{1}{9}\\
u(x,t) = f(x-t)e^{3t} + \frac{1}{3}t - \frac{1}{9}\\
\end{gather*}
Next we solve for $f(x-t)$.
\begin{align*}
u(x,0) = f(x) - \frac{1}{9} &= x^{2}\\
f(x) &= x^{2} + \frac{1}{9}
\end{align*}
Our final solution becomes
\[
u(x,t) = \left[(x-t)^{2} + \frac{1}{9}\right]e^{3t}+\frac{1}{3}t - \frac{1}{9}
\]
\newpage

\item Find the eigenvalues and eigenfunctions for the following Cauchy-Euler equation.
\[
\begin{cases*}
x^{2}y'' + xy' + \lambda^{2}y = 0\\
y(1) = y(2) = 0
\end{cases*}
\]
Since this is a Cauchy-Euler equation, we have a solution of the general form
\[
y = x^{m}
\]
By substitution, we get
\begin{align*}
& x^{2}\left[m(m-1)x^{m}\right] + x(m)x^{m-1} + \lambda^{2}x^{m} = 0\\
& x^{m}\left[m^{2} - m + m + \lambda^{2}\right] = 0\\
& m^{2} + \lambda^{2} = 0\\
& m = \pm\ \lambda i
\end{align*}
This yields the basis
\[
\left\{x^{a}\cos{(b\ln{x})}, x^{a}\sin{(b\ln{x})}\right\},
\]
which leads to the general solution
\[
y = c_{1}\cos{\lambda\ln{x}} + c_{2}\sin{\lambda\ln{x}}.
\]
Applying the boundary conditions gives us
\begin{align*}
y(1) = 0 &= c_{1}\cos{(\lambda\ln{1})} + c_{2}\sin{(\lambda\ln{1})}\\
0 &= c_{1}\cos{0} + c_{2}\sin{0}\\
0 &= c_{1}\\
y(2) = 0 &= c_{2}\sin{(\lambda\ln{2})}\\
0 &= \sin{(\lambda\ln{2})}\\
\lambda_{n}\ln{2} &= n\pi\\
\lambda_{n} &= \frac{n\pi}{\ln{2}}
\end{align*}
The corresponding eigenfunction is
\[
\phi_{n} = c_{2}\sin{\left[\frac{n\pi}{\ln{2}}\ln{x}\right]}
\]
\end{enumerate}
\end{document}
