\documentclass{article}
\usepackage{amssymb,amsmath}
\usepackage{mathtools}
\usepackage{array}
\usepackage{color}
\usepackage{graphicx}
\pagecolor{black}
\color{white}
\topmargin=-0.3in
\textheight=9.2in
\textwidth=168mm
\oddsidemargin=-0.2in
\evensidemargin=-0.2in
\title{Exam Review}
\date{}

\newcommand{\beq}{\begin{quote}}
\newcommand{\eeq}{\end{quote}}
\newcommand{\dx}{\mathop{dx}}

\begin{document}
\maketitle
\begin{enumerate}
\item Find the general solutions to the following ordinary differential equations.
\begin{enumerate}
%%%QUESTION 1.a%%%
\item $y'(t) + 4y(t) = 1 + 2t$
\beq
\begin{minipage}[t]{0.4\textwidth}
Homogeneous Solution:
\begin{gather*}
y' + 4y = 0\\
r + 4 = 0\\
r = -4\\
y_{g}(t) = ce^{-4t}
\end{gather*}
\end{minipage}
\begin{minipage}[t]{0.4\textwidth}
Particular Solution:
\begin{gather*}
y' + 4y = 1 + 2t\\
y = At + B\qquad y'= A\\
A + 4At + 4B = 1 + 2t\\
4A = 2\qquad A + 4B = 1\\
A = \frac{1}{2}\qquad B = \frac{1}{8}\\
y_{p}(t) = \frac{1}{2}t + \frac{1}{8}
\end{gather*}
\end{minipage}
\[
y(t) = ce^{-4t} + \frac{1}{2}t + \frac{1}{8}
\]
\eeq
%%%QUESTION 1.b%%%
\item $y''(t) + y(t) = \cos{\omega t}$
\beq
\begin{minipage}[t]{0.4\textwidth}
Homogeneous Solution:
\begin{gather*}
y''(t) + y(t) = 0\\
r^{2} + 1 = 0\\
r = \pm\ i\\
y_{g}(t) = c_{1}\cos{t} + c_{2}\sin{t}
\end{gather*}
\end{minipage}
\begin{minipage}[t]{0.4\textwidth}
Particular Solution:
\begin{gather*}
\end{gather*}
\end{minipage}
\eeq
\end{enumerate}
\item Here is another Question
%%%QUESTION 3%%%
\item Solve the initial boundary value problem.
\[
\begin{cases*}
u_{tt} - u_{xx} = 0\\
u(x,0) = f(x),\ u_{t}(x,0) = 0\\
u(0,t) = u(1,t) = 0
\end{cases*}
\qquad\qquad
f(x) =
\begin{cases*}
x,\qquad\quad\ 0\leq x\leq\frac{1}{2}\\
1- x\qquad \frac{1}{2}\leq x\leq 1
\end{cases*}
\]
\beq
\begin{align*}
u(x,t) &= \sum_{n=1}^{\infty}(a_{n}\cos{(n\pi t)} + b_{n}\sin{(n\pi t)})\sin{(n\pi x)}\\
u(x,0) &= \sum_{n=1}^{\infty}a_{n}\sin{(n\pi x)} = f(x)\\
u_{t}(x,0) &= \sum_{n=1}^{\infty}n\pi b_{n}\sin{(n\pi x)} = 0
\end{align*}
\begin{align*}
a_{n} &= 2\left(\int_{0}^{1}f(x)\sin{(n\pi x)}\dx\right)\\
&= 2\left(\int_{0}^{1/2}x\sin{(n\pi x)}\dx + \int_{1/2}^{1}(1-x)\sin{(n\pi x)}\dx\right)\\
&= 2\left(\int_{0}^{1/2}x\sin{(n\pi x)}\dx + \int_{1/2}^{1}\sin{(n\pi x)}\dx - \int_{1/2}^{1}x\sin{(n\pi x)}\dx\right)\\
&= 2\left(\left[\frac{\sin{(n\pi x)}}{(n\pi)^{2}} - \frac{x\cos{(n\pi x)}}{n\pi}\right]\Bigg|_{0}^{1/2} + \left[ \frac{-\cos{(n\pi x)}}{n\pi}\right]\Bigg|_{1/2}^{1} + \left[\frac{x\cos{(n\pi x)}}{n\pi} - \frac{\sin{(n\pi x)}}{(n\pi)^2}\right]\Bigg|_{1/2}^{1}\right)\\
&= 2\left(\frac{\sin{\frac{n\pi}{2}}}{(n\pi)^2} - \frac{\cos{\frac{n\pi}{2}}}{2n\pi} + \frac{\cos{\frac{n\pi}{2}}}{n\pi} - \frac{\cos{n\pi}}{n\pi} - \frac{\cos{\frac{n\pi}{2}}}{2n\pi} + \frac{\sin{\frac{n\pi}{2}}}{(n\pi)^{2}} + \frac{\cos{n\pi}}{n\pi} - \frac{\sin{n\pi}}{(n\pi)^{2}}\right)\\
&= \frac{4\sin{\frac{n\pi}{2}}}{(n\pi)^{2}}
\end{align*}
\begin{align*}
b_{n} &= \frac{\frac{1}{\pi}\int_{0}^{1}0\dx}{n\pi}\\
&= 0
\end{align*}
\[
u(x,t) = \frac{4}{\pi^{2}}\sum_{k=0}^{\infty}\frac{(-1)^{k}}{(2k+1)^{2}}\cos{(2k\pi t + \pi t)}\sin{(2k\pi t + \pi t)}
\]
\eeq


\newpage
\item Solve the following partial differential equation.
\[
\begin{cases*}
u_{t} - u_{xx} = 0\\
u(x,0) = 0\\
u(0,t) = A\cos{t},\ u(1,t) = 0
\end{cases*}
\]
\begin{align*}
\delta(x,t) &= A\cos{t} - xA\cos{t}\\
\gamma(x,t) &= u(x,t) - \delta(x,t)\\
&= u - A\cos{t} + xA\cos{t}\\
\gamma_{t}(x,t) &= u_{t} + A\sin{t} - xA\sin{t}
\end{align*}
\end{enumerate}
\end{document}
