\documentclass{article}
\usepackage{amssymb,amsmath}
\usepackage{ mathrsfs }
\usepackage{mathtools}
\usepackage{array}
\topmargin=-0.3in
\textheight=9.2in
\textwidth=168mm
\oddsidemargin=-0.2in
\evensidemargin=-0.2in
\newcommand{\Lagr}{\mathscr{L}}
\title{Laplace Transforms}
\date{}
\begin{document}
\maketitle
\[
\Lagr[f(t)] = \int_{0}^{\infty}e^{-st}f(t)\mathop{dt}
\qquad\qquad
\Lagr^{-1}[F(s)] = 2i\pi\lim_{\tau\to\infty}\int_{\gamma - i\tau}^{\gamma + i\tau}e^{st}F(s)\mathop{ds}
\]
\begin{center}
\vspace{1cm}
\begin{tabular}{c c}
$f(t) = \Lagr^{-1}[F(s)]$\qquad\qquad\qquad & \qquad\qquad\qquad$F(s) = \Lagr[f(t)]$\\
\hline \\
$1$ & $\frac{1}{s}$\\
\\
$e^{at}$ & $\frac{1}{s-a}$\\
\\
$t^{n}$ & $\frac{n!}{s^{n+1}}$\\
\\
$\sin{(at)}$ & $\frac{a}{s^{2} + a^{2}}$\\
\\
$\cos{(at)}$ & $\frac{s}{s^{2} + a^{2}}$\\
\\
$\sinh{(at)}$ & $\frac{a}{s^{2} - a^{2}}$\\
\\
$\cosh{(at)}$ & $\frac{s}{s^{2} - a^{2}}$\\
\\
$e^{at}\sin{(bt)}$ & $\frac{b}{(s-a)^{2}+b^{2}}$\\
\\
$e^{at}\cos{(bt)}$ & $\frac{s-a}{(s-a)^{2}+b^{2}}$\\
\\
$t^{n}e^{at}$ & $\frac{n!}{(s-a)^{n+1}}$\\
\\
$f'(t)$ & $sF(s) - f(0)$\\
\\
$f''(t)$ & $s^{2}F(s)-sf(0) - f'(0)$\\
\\
$\int_{0}^{t}f(t-\tau)g(\tau)\mathop{d\tau}$ & $F(s)G(s)$\\
\\
$\delta(t-c) =
\begin{cases}
\infty,\quad (t-c)=0\\
0,\quad\ (t-c)\neq 0
\end{cases}
$ & $e^{-cs}$
\end{tabular}
\end{center}
\end{document}