\documentclass{article}
\usepackage{amssymb,amsmath}
\usepackage{mathtools}
\usepackage{array}
\topmargin=-0.3in
\textheight=9.2in
\textwidth=168mm
\oddsidemargin=-0.2in
\evensidemargin=-0.2in
\title{Formal Solutions To PDE's}
\date{}
\begin{document}
\maketitle
\section{Homogeneous Solutions}
\hrule
\noindent\\
%%%HEAT EQUATION%%%
\subsection{The Heat Equation}
\begin{minipage}{0.5\textwidth}
\subsubsection*{Dirichlet}
\begin{gather*}
\begin{cases}
u_{t} - ku_{xx} = 0\\
u(0,t) = u(\ell,t) = 0\\
u(x,0) = f(x)
\end{cases}\\
u(x,t) = \sum_{n=1}^{\infty}b_{n}e^{-k\left(\frac{n\pi}{\ell}\right)^{2}t}\sin{\left(\frac{n\pi x}{\ell}\right)}\\
b_{n} = \frac{2}{\ell}\int_{0}^{\ell}f(x)\sin{\left(\frac{n\pi x}{\ell}\right)}\mathop{dx}
\end{gather*}
\noindent\\\\\\
\end{minipage}
\begin{minipage}{0.5\textwidth}
\subsubsection*{Neumann}
\begin{gather*}
\begin{cases}
u_{t} - ku_{xx} = 0\\
u_{x}(0,t) = u_{x}(\ell,t) = 0\\
u(x,0) = f(x)
\end{cases}\\
u(x,t) = \frac{a_{0}}{2} + \sum_{n=1}^{\infty}a_{n}e^{-k\left(\frac{n\pi}{\ell}\right)^{2}t}\cos{\left(\frac{n\pi x}{\ell}\right)}\\
a_{n} = \frac{2}{\ell}\int_{0}^{\ell}f(x)\cos{\left(\frac{n\pi x}{\ell}\right)}\mathop{dx}\\
a_{0} = \frac{2}{\ell}\int_{0}^{\ell}f(x)\mathop{dx}\\
\end{gather*}
\end{minipage}

\subsubsection*{Robin}
\begin{minipage}{0.5\textwidth}
\begin{gather*}
\begin{cases}
u_{t} - ku_{xx} = 0\\
u(0,t) = u_{x}(\ell,t) = 0\\
u(x,0) = f(x)
\end{cases}\\
u(x,t) = \sum_{n=1}^{\infty}a_{n}e^{-k\left(\left[n + \frac{1}{2}\right]\frac{\pi}{\ell}\right)^{2}t}\sin{\left(\left[n + \frac{1}{2}\right]\frac{\pi}{\ell}\right)}\\
a_{n} = \frac{2}{\ell}\int_{0}^{\ell}f(x)\sin{\left(\left[n + \frac{1}{2}\right]\frac{\pi}{\ell}\right)}\mathop{dx}\\
\end{gather*}
\end{minipage}
\begin{minipage}{0.5\textwidth}
\begin{gather*}
\begin{cases}
u_{t} - ku_{xx} = 0\\
u_{x}(0,t) = u(\ell,t) = 0\\
u(x,0) = f(x)
\end{cases}\\
u(x,t) = \sum_{n=1}^{\infty}a_{n}e^{-k\left(\left[n + \frac{1}{2}\right]\frac{\pi}{\ell}\right)^{2}t}\cos{\left(\left[n + \frac{1}{2}\right]\frac{\pi}{\ell}\right)}\\
a_{n} = \frac{2}{\ell}\int_{0}^{\ell}f(x)\cos{\left(\left[n + \frac{1}{2}\right]\frac{\pi}{\ell}\right)}\mathop{dx}\\
\end{gather*}
\end{minipage}


%%%WAVE EQUATION%%%
\subsection{The Wave Equation}
\subsubsection*{Dirichlet}
\begin{gather*}
\begin{cases}
u_{tt} - c^{2}u_{xx} = 0\\
u(0,t) = u(\ell,t) = 0\\
u(x,0) = f(x),\ u_{t}(x,0) = g(x)
\end{cases}\\
u(x,t) = \sum_{n=1}^{\infty}\left[a_{n}\cos{\left(\frac{n\pi c t}{\ell}\right)} + b_{n}\sin{\left(\frac{n\pi c t}{\ell}\right)}\right]\sin{\left(\frac{n\pi x}{\ell}\right)}\\
a_{n} = \frac{2}{\ell}\int_{0}^{\ell}f(x)\sin{\left(\frac{n\pi x}{\ell}\right)}\mathop{dx}\\
b_{n} = \frac{2}{n\pi c}\int_{0}^{\ell}g(x)\sin{\left(\frac{n\pi x}{\ell}\right)}\mathop{dx}\\
\end{gather*}

\subsubsection*{Neumann}
\begin{gather*}
\begin{cases}
u_{tt} - c^{2}u_{xx} = 0\\
u_{x}(0,t) = u_{x}(\ell,t) = 0\\
u(x,0) = f(x),\ u_{t}(x,0) = g(x)
\end{cases}\\
u(x,t) = \frac{a_{0}}{2} + \frac{b_{0}}{2}t +\sum_{n=1}^{\infty}\left[a_{n}\cos{\left(\frac{n\pi c t}{\ell}\right)} + b_{n}\sin{\left(\frac{n\pi c t}{\ell}\right)}\right]\cos{\left(\frac{n\pi x}{\ell}\right)}\\
a_{n} = \frac{2}{\ell}\int_{0}^{\ell}f(x)\cos{\left(\frac{n\pi x}{\ell}\right)}\mathop{dx}\qquad\qquad
a_{0} = \frac{2}{\ell}\int_{0}^{\ell}f(x)\mathop{dx}\\
b_{n} = \frac{2}{n\pi c}\int_{0}^{\ell}g(x)\cos{\left(\frac{n\pi x}{\ell}\right)}\mathop{dx}\qquad\qquad
b_{0} = \frac{2}{n\pi c}\int_{0}^{\ell}g(x)\mathop{dx}\\
\end{gather*}

\subsubsection*{Robin}
\begin{gather*}
\begin{cases}
u_{tt} - c^{2}u_{xx} = 0\\
u(0,t) = u_{x}(\ell,t) = 0\\
u(x,0) = f(x),\ u_{t}(x,0) = g(x)
\end{cases}\\
u(x,t) = a_{0} + b_{0}t +\sum_{n=1}^{\infty}\left[a_{n}\cos{\left(\left[n + \frac{1}{2}\right]\frac{\pi t}{\ell}\right)} + b_{n}\sin{\left(\left[n + \frac{1}{2}\right]\frac{\pi t}{\ell}\right)}\right]\sin{\left(\left[n + \frac{1}{2}\right]\frac{\pi x}{\ell}\right)}\\
a_{n} = \frac{2}{\ell}\int_{0}^{\ell}f(x)\sin{\left(\left[n + \frac{1}{2}\right]\frac{\pi x}{\ell}\right)}\mathop{dx}\qquad\qquad
a_{0} = \frac{2}{\ell}\int_{0}^{\ell}f(x)\mathop{dx}\\
b_{n} = \frac{2}{n\pi c}\int_{0}^{\ell}g(x)\sin{\left(\left[n + \frac{1}{2}\right]\frac{\pi x}{\ell}\right)}\mathop{dx}\qquad\qquad
b_{0} = \frac{2}{n\pi c}\int_{0}^{\ell}g(x)\mathop{dx}\\
\end{gather*}
\begin{gather*}
\begin{cases}
u_{tt} - c^{2}u_{xx} = 0\\
u_{x}(0,t) = u(\ell,t) = 0\\
u(x,0) = f(x),\ u_{t}(x,0) = g(x)
\end{cases}\\
u(x,t) = a_{0} + b_{0}t +\sum_{n=1}^{\infty}\left[a_{n}\cos{\left(\left[n + \frac{1}{2}\right]\frac{\pi t}{\ell}\right)} + b_{n}\sin{\left(\left[n + \frac{1}{2}\right]\frac{\pi t}{\ell}\right)}\right]\cos{\left(\left[n + \frac{1}{2}\right]\frac{\pi x}{\ell}\right)}\\
a_{n} = \frac{2}{\ell}\int_{0}^{\ell}f(x)\cos{\left(\left[n + \frac{1}{2}\right]\frac{\pi x}{\ell}\right)}\mathop{dx}\qquad\qquad
a_{0} = \frac{2}{\ell}\int_{0}^{\ell}f(x)\mathop{dx}\\
b_{n} = \frac{2}{n\pi c}\int_{0}^{\ell}g(x)\cos{\left(\left[n + \frac{1}{2}\right]\frac{\pi x}{\ell}\right)}\mathop{dx}\qquad\qquad
b_{0} = \frac{2}{n\pi c}\int_{0}^{\ell}g(x)\mathop{dx}\\
\end{gather*}

%%%LAPLACE EQUATION%%%
\subsection{Laplace Equation}
\subsubsection*{Rectangular Region}
\paragraph{Dirichlet}
\begin{gather*}
\begin{cases}
u_{xx} + u_{yy} = 0\\
u(0,y) = u(\ell,y) = 0
\end{cases}\\
u(x,y) = \sum_{n=1}^{\infty}\left[b_{n}\sinh{\left(\frac{n\pi y}{\ell}\right)} + a_{n}\cosh{\left(\frac{n\pi y}{\ell}\right)}\right]\sin{\left(\frac{n\pi x}{\ell}\right)}
\end{gather*}

\paragraph{Neumann}
\begin{gather*}
\begin{cases}
u_{xx} + u_{yy} = 0\\
u_{x}(0,y) = u_{x}(\ell,y) = 0
\end{cases}\\
u(x,y) = a_{0} + b_{0}y + \sum_{n=1}^{\infty}\left[b_{n}\sinh{\left(\frac{n\pi y}{\ell}\right)} + a_{n}\cosh{\left(\frac{n\pi y}{\ell}\right)}\right]\cos{\left(\frac{n\pi x}{\ell}\right)}
\end{gather*}

\paragraph{Robin}
\begin{gather*}
\begin{cases}
u_{xx} + u_{yy} = 0\\
u(0,y) = u_{x}(\ell,y) = 0
\end{cases}\\
u(x,y) = \sum_{n=1}^{\infty}\left[b_{n}\sinh{\left(\left[n + \frac{1}{2}\right]\frac{\pi y}{\ell}\right)} + a_{n}\cosh{\left(\left[n + \frac{1}{2}\right]\frac{\pi y}{\ell}\right)}\right]\sin{\left(\left[n + \frac{1}{2}\right]\frac{\pi x}{\ell}\right)}
\end{gather*}
\begin{gather*}
\begin{cases}
u_{xx} + u_{yy} = 0\\
u_{x}(0,y) = u(\ell,y) = 0
\end{cases}\\
u(x,y) = \sum_{n=1}^{\infty}\left[b_{n}\sinh{\left(\left[n + \frac{1}{2}\right]\frac{\pi y}{\ell}\right)} + a_{n}\cosh{\left(\left[n + \frac{1}{2}\right]\frac{\pi y}{\ell}\right)}\right]\cos{\left(\left[n + \frac{1}{2}\right]\frac{\pi x}{\ell}\right)}
\end{gather*}

\subsubsection*{Circular Region}
\begin{gather*}
\begin{cases}
u_{rr} + \frac{1}{r}u_{r} + \frac{1}{r^{2}}u_{\theta\theta} = 0\\
u(h,\theta)  = f(\theta)
\end{cases}\\
u(r,\theta) = \frac{a_{0}}{2} + \sum_{n=1}^{\infty}a_{n}\frac{r^{n}}{a^{n}}\cos{(n\theta)} + b_{n}\frac{r^{n}}{a^{n}}\sin{(n\theta)}\\
a^{n}a_{n} = \int_{-\pi}^{\pi}f(\theta)\cos{(n\theta)}\mathop{d\theta}\\
a^{n}b_{n} = \int_{-\pi}^{\pi}f(\theta)\sin{(n\theta)}\mathop{d\theta}
\end{gather*}
\newpage




\section{Non-Homogeneous Solutions}
\hrule
\noindent\\
%%%HEAT EQUATION%%%
\subsection{The Heat Equation}
\begin{minipage}{0.5\textwidth}
\subsubsection*{Dirichlet}
\begin{gather*}
\begin{cases}
u_{t} - ku_{xx} = h(x,t)\\
u(0,t) = u(\ell,t) = 0\\
u(x,0) = f(x)
\end{cases}\\
u(x,t) = \sum_{n=1}^{\infty}b_{n}(t)\sin{\left(\frac{n\pi x}{\ell}\right)}\\
%b_{n}(t) = \frac{2}{\ell}\int_{0}^{\ell}h(x,t)\sin{\left(\frac{n\pi x}{\ell}\right)}\mathop{dx}\\
\sum_{n=1}^{\infty}\left[b_{n}^{'}(t)+k\left(\frac{n\pi}{\ell}\right)^{2}b_{n}(t)\right]\sin{\left(\frac{n\pi x}{\ell}\right)} = h(x,t)
\end{gather*}
\end{minipage}
\begin{minipage}{0.5\textwidth}
\subsubsection*{Neumann}
\begin{gather*}
\begin{cases}
u_{t} - ku_{xx} = h(x,t)\\
u_{x}(0,t) = u_{x}(\ell,t) = 0\\
u(x,0) = f(x)
\end{cases}\\
u(x,t) = \frac{a_{0}(t)}{2} + \sum_{n=1}^{\infty}a_{n}(t)\cos{\left(\frac{n\pi x}{\ell}\right)}\\
\frac{a_{0}'(t)}{2} + \sum_{n=1}^{\infty}\left[a_{n}'(t) + k\left(\frac{n\pi}{\ell}\right)^{2}a_{n}\right]\cos{\left(\frac{n\pi x}{\ell}\right)} = h(x,t)
\end{gather*}
\end{minipage}
%%%WAVE EQUATION%%%
\subsection{The Wave Equation}
\begin{minipage}{0.5\textwidth}
\subsubsection*{Dirichlet}
\begin{gather*}
\begin{cases}
u_{tt} - c^{2}u_{xx} = h(x,t)\\
u(0,t) = u(\ell,t) = 0\\
u(x,t) = f(x),\ u_{t}(x,0) = g(x) 
\end{cases}\\
u(x,t) = \sum_{n=1}^{\infty}b_{n}(t)\sin{\left(\frac{n\pi x}{\ell}\right)}\\
\sum_{n=1}^{\infty}\left[b_{n}''(t) + \left(\frac{n\pi}{\ell}\right)^{2}b_{n}(t)\right]\sin{\left(\frac{n\pi x}{\ell}\right)} = h(x,t)
\end{gather*}
\end{minipage}
\begin{minipage}{0.5\textwidth}
\subsubsection*{Neumann}
\begin{gather*}
\begin{cases}
u_{tt} - c^{2}u_{xx} = h(x,t)\\
u_{x}(0,t) = u_{x}(\ell,t) = 0\\
u(x,t) = f(x),\ u_{t}(x,0) = g(x) 
\end{cases}\\
u(x,t) = \frac{b_{0}(t)}{2} + \sum_{n=1}^{\infty}b_{n}(t)\cos{\left(\frac{n\pi x}{\ell}\right)}\\
\frac{b_{0}''(t)}{2} + \sum_{n=1}^{\infty}\left[b_{n}''(t) + \left(\frac{n\pi}{\ell}\right)^{2}b_{n}(t)\right]\cos{\left(\frac{n\pi x}{\ell}\right)} = h(x,t)
\end{gather*}
\end{minipage}

\subsection{Non-Homogeneous Boundaries}
\begin{gather*}
\begin{cases}
u_{t} - ku_{xx} = h(x,t)\\
u(0,t) = L(t),\ u(\ell,t) = R(t)\\
u(x,0) = f(x)
\end{cases}
\hspace{2cm}
\begin{cases}
u_{t} - ku_{xx} = h(x,t)\\
u(0,t) = L(t),\ u(\ell,t) = R(t)\\
u(x,0) = f(x)
\end{cases}\\
\delta(x,t) = L + \frac{x}{\ell}(R - L)\\
\gamma(x,t) = u(x,t) - \delta(x,t)
\end{gather*}



\newpage
\section{Cauchy Problems}
\hrule
\noindent\\
%%%HEAT EQUATION%%%
\subsection{The Heat Equation}
\subsubsection*{Homogeneous}
\begin{gather*}
\begin{cases}
u_{t} - k u_{xx} = 0\\
u(x,0) = f(x)
\end{cases}\\
u(x,t) = \frac{1}{\sqrt{4k\pi t}}\int_{-\infty}^{\infty}e^{\frac{-(x-y)^{2}}{4kt}}f(y)\mathop{dy}
\end{gather*}
\subsubsection*{Non-Homogeneous}
\begin{gather*}
\begin{cases}
u_{t} - k u_{xx} = h(x,t)\\
u(x,0) = f(x)
\end{cases}\\
u(x,t) = \frac{1}{\sqrt{4k\pi t}}\int_{-\infty}^{\infty}e^{\frac{-(x-y)^{2}}{4kt}}f(y)\mathop{dy} + \int_{0}^{t}\int_{-\infty}^{\infty}\frac{1}{\sqrt{4k\pi(t-s)}}e^{\frac{-(x-y)^{2}}{4k(t -s)}}h(y,s)\mathop{dy}\mathop{ds}
\end{gather*}
%%%WAVE EQUATION%%%
\subsection{The Wave Equation}
\subsubsection*{Homogeneous}
\begin{gather*}
\begin{cases}
u_{tt} - c^{2}u_{xx} = 0\\
u(x,0) = f(x),\ u_{t}(x,0) = g(x)
\end{cases}\\
u(x,t) = \frac{1}{2}\left[f(x+ct) + f(x-ct)\right] + \frac{1}{2c}\int_{x-ct}^{x+ct}g(s)\mathop{ds}
\end{gather*}
\subsubsection*{Non-Homogeneous}
\begin{gather*}
\begin{cases}
u_{tt} - c^{2}u_{xx} = h(x,t)\\
u(x,0) = f(x),\ u_{t}(x,0) = g(x)
\end{cases}\\
u(x,t) = \frac{1}{2}\left[f(x+ct) + f(x-ct)\right] + \frac{1}{2c}\int_{x-ct}^{x+ct}g(s)\mathop{ds} + \frac{1}{2c}\int_{0}^{t}\int_{x-c(t-s)}^{x+c(t-s)}h(y,s)\mathop{dy}\mathop{ds}
\end{gather*}
\end{document}